\documentclass{article}
\usepackage{amsmath}
\usepackage[a4paper, margin=1in]{geometry}

\title{Analytic Test of RT-GSFit}
\author{Alexander Prokopyszyn}
\date{May 2025}

\begin{document}

\maketitle

\section{Deriving Bessel's Eqn from the Grad-Shafranov Eqn}

The Grad-Shafranov equation is given by
\[\frac{\partial^2 \psi}{\partial R^2} - \frac{1}{R}\frac{\partial \psi}{\partial R} + \frac{\partial^2 \psi}{\partial z^2} = -\mu_oR^2p'(\psi) - F(\psi)F'(\psi).\]
We will assume a plasma beta, $\beta=0$. We are interested in solving the Grad-Shafranov equation inside the LCFS. 
% Let $R=R_o$, $z=z_o$ be the coordinates of the o-point. 
% We will assume that
% \[\frac{|R-R_o|}{R_o} = O(\epsilon),\]
% \[R\frac{\partial}{\partial R} = O\left(\frac{1}{\epsilon}\right)\]
% \[R\frac{\partial}{\partial z} = O\left(\frac{1}{\epsilon}\right)\]
% \[\frac{|R-R_o|}{R_o} \ll 1,\]
% \[\implies \frac{1}{R} = \frac{1}{R-R_0 + R_0} = \frac{1}{R_0}\left(\frac{1}{1+\frac{R-R_0}{R}}\right)\]
We will take the large aspect-ratio limit and assume $R\rightarrow \infty$.
Hence, we can simplify the Grad-Shafranov to
\[\frac{\partial^2 \psi}{\partial R^2} + \frac{\partial^2 \psi}{\partial z^2} = -F(\psi)F'(\psi).\]
We will assume poloidal symmetry, and so we assume $\psi=\psi(\rho)$.
Let
\[\rho = \sqrt{(R-R_o)^2+(z-z_o)^2}.\]
\[R-R_o = \rho\cos(\theta),\]
\[z-z_o = \rho \sin(\theta),\]
% \[\theta = \tan^{-1}(z-z_o, R-R_o)\]
\[\mathbf{\hat{\rho}} = \cos(\theta) \mathbf{\hat{R}} + \sin(\theta)\mathbf{\hat{z}},\]
\[\mathbf{\hat{\theta}} = -\sin(\theta) \mathbf{\hat{R}} + \cos(\theta)\mathbf{\hat{z}}.\]
Note that
\[\begin{aligned}
\frac{\partial \psi}{\partial R} &= \frac{\partial \rho}{\partial R}\frac{d \psi}{d \rho} \\
&= \frac{(R-R_o)}{\sqrt{(R-R_o)^2+(z-z_o)^2}}\frac{d \psi}{d \rho} \\
&= \cos(\theta)\frac{d \psi}{d \rho},
\end{aligned}\]
\[\begin{aligned}
\frac{\partial \psi}{\partial z} &= \frac{\partial \rho}{\partial z}\frac{d \psi}{d \rho} \\
&= \frac{(z-z_o)}{\sqrt{(R-R_o)^2+(z-z_o)^2}}\frac{d \psi}{d \rho} \\
&= \sin(\theta)\frac{d \psi}{d \rho},
\end{aligned}\]
\[\begin{aligned}
    \frac{\partial \psi}{\partial R}\mathbf{\hat{R}} + \frac{\partial \psi}{\partial z}\mathbf{\hat{z}} &= \frac{d \psi}{d \rho}(\cos(\theta) \mathbf{\hat{R}} + \sin(\theta)\mathbf{\hat{z}}) \\
    &= \frac{d \psi}{d \rho}\mathbf{\hat{\rho}},
\end{aligned}
\]
\[\begin{aligned}
\mathbf{\hat{R}}\cdot\frac{\partial \mathbf{\hat{\rho}}}{\partial R} &= \frac{\partial}{\partial R}\left(\frac{R-R_o}{\sqrt{(R-R_o^2)+(z-z_o^2)}}\right)\\
&= \frac{\sin^2\theta}{\rho}
\end{aligned}\]
\[\begin{aligned}
\mathbf{\hat{z}}\cdot\frac{\partial \mathbf{\hat{\rho}}}{\partial z} &= \frac{\partial}{\partial z}\left(\frac{z-R_o}{\sqrt{(R-R_o^2)+(z-z_o^2)}}\right)\\
&= \frac{\cos^2\theta}{\rho}
\end{aligned}\]
\[\begin{aligned}
\frac{\partial^2\psi}{\partial R^2} + \frac{\partial^2 \psi}{\partial z^2} &= \left(\mathbf{\hat{R}}\frac{\partial }{\partial R} + \mathbf{\hat{z}}\frac{\partial }{\partial z}\right)
\cdot\left(\frac{\partial \psi}{\partial R}\mathbf{\hat{R}} + \frac{\partial \psi}{\partial z}\mathbf{\hat{z}}\right) \\ 
&= \left(\mathbf{\hat{R}}\frac{\partial }{\partial R} + \mathbf{\hat{z}}\frac{\partial }{\partial z}\right) \cdot \left(\frac{d \psi}{d \rho}\mathbf{\hat{\rho}}\right) \\
&= \cos(\theta)\frac{\partial}{\partial R}\left(\frac{d \psi}{d \rho}\right)
+ \frac{d \psi}{d \rho}\mathbf{\hat{R}}\cdot\frac{\partial \mathbf{\hat{\rho}}}{\partial R}
+ \sin(\theta)\frac{\partial}{\partial z}\left(\frac{d \psi}{d \rho}\right)
+ \frac{d \psi}{d \rho}\mathbf{\hat{z}}\cdot\frac{\partial \mathbf{\hat{\rho}}}{\partial z} \\
&= \frac{d^2\psi}{d \rho^2} + \frac{1}{\rho}\frac{d \psi}{d \rho}.
\end{aligned}\]
Hence,
we can rewrite the Grad-Shafranov equation as
\[\frac{d^2\psi}{d \rho^2} + \frac{1}{\rho}\frac{d \psi}{d \rho} = -F(\psi)F'(\psi).\]

RTGSFit assumes $FF'$ is of the form
\[FF' = a(1-\psi_N),\]
where $a$ is a constant and
\[\psi_N = \frac{\psi_o-\psi}{\psi_o-\psi_b},\]
where $\psi_b$ is $\psi$ at the last closed flux surface and $\psi_o$ is the value of $\psi$ at the o-point.
Let
\[\psi(\rho)=\psi'(\rho)+\psi_b,\]
\[a'=\frac{a}{(\psi_o - \psi_b)},\]
hence by substituting our expression for $\psi$ in terms of $\psi'$ and $a$ in terms of a' we get
\[\frac{d^2\psi'}{d \rho^2} + \frac{1}{\rho}\frac{d \psi'}{d \rho} = -a'\psi'.\]
Multiplying through by $\rho^2$ and rearranging we arrive at an equation that is nearly Bessel's equation of order 0
\[\rho^2\frac{d^2\psi'}{d \rho^2} + \rho\frac{d \psi'}{d \rho} + a'\rho^2\psi'= 0.\]
Let 
\[s=\frac{a'}{|a'|}\sqrt{|a'|}\rho,\]
\[\implies \rho=\frac{a'}{|a'|}\frac{1}{\sqrt{|a'|}}s\]
\[\implies \frac{\partial }{\partial \rho} =\frac{a'}{|a'|}\sqrt{|a'|}\frac{\partial }{\partial s},\]
\[\implies \frac{\partial^2 }{\partial \rho^2} =a'\frac{\partial^2 }{\partial s^2},\]
\[\implies \rho^2 = \frac{s^2}{a'}\]
Hence, the Grad-Shafranov equation becomes
\[s^2\frac{\partial^2\psi'}{\partial s^2} + s\frac{\partial \psi'}{\partial s} + s^2\psi'= 0,\]
which is exactly of the same form as Bessel's equation of order 0.

\section{Solving Bessels' equation}

We know that $\psi'$ is of the form
\[\psi' = C_1J_0(s) + C_2Y_0(s),\]
where $J_0$ and $Y_0$ are Bessel function of order zero of the first and second kind respectively. We know that $\psi$ is finite at $R=R_o$, $z=z_o$, hence, $C_2=0$.
Past the last closed flux surface, there is no plasma current. 
Hence, the full solution for $\psi'$ is
\[\psi'(\rho) = C_1J_0(\sqrt{a'}\rho).\]
Note that RT-GSFit assumes $\psi$ is a monotonically decreasing function away from the o-point inside the LCFS, but $J_0(\sqrt{a'}\rho)$ oscillates. This means the corodinate of the LCFS, $\rho=\rho_b$, must be less than the value of $\rho$ where $J_0(\sqrt{a'}\rho)$ has its first turning point (besides the turning point at $\rho=0$). Note that
\[\frac{d }{d x}J_0(x) = -J_1(x),\]
and $J_1(x)$ has its first root at about $x=\pm3.8317$ (besides the root at $x=0$). Hence, we require
\[\sqrt{a'}\rho < 3.8317 \implies \rho < \frac{3.8317}{\sqrt{a'}}.\]

Note that
\[a = \frac{\psi_o-\psi_b}{\rho_b^2}.\]

\section{Tidying up solution}

Without loss of generality, we will set $\psi_b=0$. Hence
\[\psi = \psi_oJ_0\left(\sqrt{\frac{a}{\psi_o}}\rho\right).\]
Let
\[a = \frac{\psi_o}{\rho_b^2}(a^*)^2,\]
where $a^*>0$,
\[\implies a^* = \sqrt{\frac{a\rho_b^2}{\psi_o}}.\]
Hence,
\[\psi = \psi_oJ_0\left(a^*\frac{\rho}{\rho_b}\right).\]
Since $\psi(\rho_b)=\psi_b=0$ we know that
\[J_0(a^*)=0,\]
\[\implies a^* \approx 2.404825557695772768621631879326454643124244909146\]

\section{Solution for $\rho>\rho_b$}

For $\rho>\rho_b$ there is no plasma current and the Grad-Shafranov equation is given by
\[\rho^2\frac{d^2\psi}{d \rho^2} + \rho\frac{d \psi}{d \rho} = 0\]
and we require
\[\psi(\rho_b)=0.\]
The equation has the general solution
\[\psi = C_1\ln\left(\frac{\rho}{\rho_b}\right).\]
We also require continuity of the derivative of $\psi$, note that
\[\frac{d}{d\rho}\left[\psi_oJ_0\left(a^*\frac{\rho}{\rho_b}\right)\right]=-\frac{\psi_oa^*}{\rho_b}J_1\left(a^*\frac{\rho}{\rho_b}\right),\]
\[\frac{d}{d\rho} C_1\ln\left(\frac{\rho}{\rho_b}\right) = \frac{C_1}{\rho},\]
hence,
\[\frac{C_1}{\rho_b} = -\frac{\psi_oa^*}{\rho_b}J_1(a^*),\]
\[\implies C_1 = -\psi_oa^*J_1(a^*),\]
% Note that
% \[J_1(a^*) \approx 0.519147497289466788140202640208624244569819046868.\]
Hence, for $r\ge\rho_b$
\[\psi = -\psi_oa^*J_1(a^*)\ln\left(\frac{\rho}{\rho_b}\right).\]



% then
% \[\begin{aligned}
% \frac{\partial }{\partial R} &= \frac{\partial \rho}{\partial R}\frac{\partial}{\partial \rho} + \frac{\partial \theta}{\partial R}\frac{\partial}{\partial \theta} \\
% &= \frac{(R-R_o)}{\sqrt{(R-R_o)^2+(z-z_o)^2}}\frac{\partial}{\partial \rho}-\frac{z-z_o}{(R-R_o)^2+(z-z_o)^2}\frac{\partial}{\partial \rho}
% \end{aligned}\]
% \[\begin{aligned}
% \frac{\partial }{\partial z} &= \frac{\partial \rho}{\partial R}\frac{\partial}{\partial \rho} + \frac{\partial \theta}{\partial R}\frac{\partial}{\partial \theta} \\
% &= \frac{(R-R_o)}{\sqrt{(R-R_o)^2+(z-z_o)^2}}\frac{\partial}{\partial \rho}-\frac{z-z_o}{(R-R_o)^2+(z-z_o)^2}\frac{\partial}{\partial \rho}
% \end{aligned}\]

\end{document}
